isabelle_code/Automata/implementation/NFA_set_spec.thy
@@ -1,0 +1,179 @@
+
+section \<open> Interface for NFAs and DFAs \<close>
+
+theory NFA_set_spec
+ 
+imports Main 
+  "../DFA" 
+  "Collections.Collections"
+
+begin
+type_synonym ('q,'a,'nfa) nfa_\<alpha> = "'nfa \<Rightarrow> ('q, 'a) NFA_rec"
+
+  locale nfa =
+    fixes \<alpha> :: "('q,'a,'nfa) nfa_\<alpha>"
+    fixes invar :: "'nfa \<Rightarrow> bool"
+    assumes nfa_is_wellformed: "invar n \<Longrightarrow> NFA (\<alpha> n)"
+
+
+
+locale nfa_determinise = n1: nfa \<alpha>1 invar1 + n2: nfa \<alpha>2 invar2    
+    for \<alpha>1 :: "('q1::{NFA_states},'a::linorder,'nfa1) nfa_\<alpha>" and invar1 and
+        \<alpha>2 :: "('q2,'a,'nfa2) nfa_\<alpha>" and invar2  and
+        T  :: "'nfa1 \<Rightarrow> (('q \<times> 'b \<times> 'q) set)" and
+        sem :: "'b \<Rightarrow> 'a set" and
+        canonical_op :: "'b \<Rightarrow> bool" and
+        intersect_op :: "'b \<Rightarrow> 'b \<Rightarrow> 'b" and
+        empty_op :: "'b \<Rightarrow> bool" 
+        +
+    fixes determinise :: "'nfa1 \<Rightarrow> 'nfa2"
+    assumes determinise_correct_aux:
+      "invar1 n \<Longrightarrow> (\<forall> (q, a, q') \<in> (T n). canonical_op a) \<Longrightarrow>
+        (\<forall> (q, a, q') \<in> (T n). sem a \<noteq> {}) \<Longrightarrow>
+      (\<forall> (q1, a1, q1') \<in> (T n). \<forall> (q2, a2, q2') \<in> (T n).
+                   a1 \<noteq> a2 \<longrightarrow> empty_op (intersect_op a1 a2))
+       \<Longrightarrow> invar2 (determinise n) \<and> 
+       NFA_isomorphic_wf (\<alpha>2 (determinise n)) (efficient_determinise_NFA (\<alpha>1 n))"
+  begin
+    lemma determinise_correct:
+      "invar1 n \<Longrightarrow> (\<forall> (q, a, q') \<in> (T n). canonical_op a)
+       \<Longrightarrow> (\<forall> (q, a, q') \<in> (T n). sem a \<noteq> {}) \<Longrightarrow>
+       (\<forall> (q1, a1, q1') \<in> (T n). \<forall> (q2, a2, q2') \<in> (T n).
+                   a1 \<noteq> a2 \<longrightarrow> empty_op (intersect_op a1 a2)) \<Longrightarrow> invar2 (determinise n)"
+      "invar1 n \<Longrightarrow> (\<forall> (q, a, q') \<in> (T n). canonical_op a)
+       \<Longrightarrow> (\<forall> (q, a, q') \<in> (T n). sem a \<noteq> {}) \<Longrightarrow>
+      (\<forall> (q1, a1, q1') \<in> (T n). \<forall> (q2, a2, q2') \<in> (T n).
+                   a1 \<noteq> a2 \<longrightarrow> empty_op (intersect_op a1 a2)) \<Longrightarrow> 
+      NFA_isomorphic_wf (\<alpha>2 (determinise n)) (efficient_determinise_NFA (\<alpha>1 n))"
+      using determinise_correct_aux by (simp_all)
+
+    lemma determinise_correct___isomorphic:
+      "invar1 n \<Longrightarrow> (\<forall> (q, a, q') \<in> (T n). canonical_op a)
+       \<Longrightarrow> (\<forall> (q, a, q') \<in> (T n). sem a \<noteq> {}) \<Longrightarrow> 
+          (\<forall> (q1, a1, q1') \<in> (T n). \<forall> (q2, a2, q2') \<in> (T n).
+                   a1 \<noteq> a2 \<longrightarrow> empty_op (intersect_op a1 a2)) \<Longrightarrow> invar2 (determinise n)"
+      "invar1 n \<Longrightarrow> (\<forall> (q, a, q') \<in> (T n). canonical_op a)
+       \<Longrightarrow> (\<forall> (q, a, q') \<in> (T n). sem a \<noteq> {}) \<Longrightarrow> 
+        (\<forall> (q1, a1, q1') \<in> (T n). \<forall> (q2, a2, q2') \<in> (T n).
+                   a1 \<noteq> a2 \<longrightarrow> empty_op (intersect_op a1 a2)) \<Longrightarrow> 
+            NFA_isomorphic_wf (\<alpha>1 n) \<A> \<and> (\<I> (\<alpha>1 n) \<noteq> {})\<Longrightarrow> 
+       NFA_isomorphic_wf (\<alpha>2 (determinise n)) (efficient_determinise_NFA \<A>)"
+      apply (simp add: determinise_correct)
+      apply (insert determinise_correct(2)[of n]
+                    NFA_isomorphic_efficient_determinise [of "\<alpha>1 n" \<A>])
+      using NFA_set.NFA_isomorphic_wf_trans apply blast
+    done
+
+    lemma determinise_correct___same:
+      "invar1 n \<Longrightarrow> (\<forall> (q, a, q') \<in> (T n). canonical_op a)
+       \<Longrightarrow> (\<forall> (q, a, q') \<in> (T n). sem a \<noteq> {}) \<Longrightarrow> 
+        (\<forall> (q1, a1, q1') \<in> (T n). \<forall> (q2, a2, q2') \<in> (T n).
+                   a1 \<noteq> a2 \<longrightarrow> empty_op (intersect_op a1 a2)) \<Longrightarrow> invar2 (determinise n)"
+      "invar1 n \<Longrightarrow> (\<forall> (q, a, q') \<in> (T n). canonical_op a)
+       \<Longrightarrow> (\<forall> (q, a, q') \<in> (T n). sem a \<noteq> {}) \<Longrightarrow> 
+        uniq_label_NFA (\<alpha>1 n) \<and> \<I> (\<alpha>1 n) \<noteq> {} \<Longrightarrow> (\<forall> (q1, a1, q1') \<in> (T n). \<forall> (q2, a2, q2') \<in> (T n).
+                   a1 \<noteq> a2 \<longrightarrow> empty_op (intersect_op a1 a2)) \<Longrightarrow>
+                    NFA_isomorphic_wf (\<alpha>2 (determinise n)) (NFA_determinise (\<alpha>1 n))"
+       using determinise_correct [of n] n1.nfa_axioms[unfolded nfa_def]
+             NFA_determinise_isomorphic_wf [of "\<alpha>1 n"]
+       by (simp_all, metis NFA_isomorphic_wf_trans)
+
+    lemma determinise_correct___same_isomorphic:
+      "invar1 n \<Longrightarrow> (\<forall> (q, a, q') \<in> (T n). canonical_op a)
+       \<Longrightarrow>(\<forall> (q, a, q') \<in> (T n). sem a \<noteq> {}) \<Longrightarrow> (\<forall> (q1, a1, q1') \<in> (T n). \<forall> (q2, a2, q2') \<in> (T n).
+                   a1 \<noteq> a2 \<longrightarrow> empty_op (intersect_op a1 a2)) \<Longrightarrow> invar2 (determinise n)"
+      "invar1 n \<Longrightarrow> (\<forall> (q, a, q') \<in> (T n). canonical_op a)
+       \<Longrightarrow> (\<forall> (q, a, q') \<in> (T n). sem a \<noteq> {}) \<Longrightarrow> (\<forall> (q1, a1, q1') \<in> (T n). \<forall> (q2, a2, q2') \<in> (T n).
+                   a1 \<noteq> a2 \<longrightarrow> empty_op (intersect_op a1 a2)) \<Longrightarrow> NFA_isomorphic_wf (\<alpha>1 n) \<A> \<Longrightarrow> 
+       uniq_label_NFA \<A> \<and> \<I> \<A> \<noteq> {} \<Longrightarrow>
+       NFA_isomorphic_wf (\<alpha>2 (determinise n)) (NFA_determinise \<A>)"
+      apply (simp add: determinise_correct)
+      apply (insert determinise_correct___isomorphic(2)[of n \<A>]
+                    NFA_determinise_isomorphic_wf [of \<A>])
+      apply (simp)
+      apply (subgoal_tac "\<I> (\<alpha>1 n) \<noteq> {}")
+      apply (metis NFA_isomorphic_wf_trans NFA_isomorphic_wf_alt_def)
+      unfolding NFA_isomorphic_wf_def NFA_isomorphic_def
+      apply fastforce
+    done
+  end
+
+
+locale nfa_complement = nfa \<alpha> invar   
+    for \<alpha> :: "('q,'a,'nfa) nfa_\<alpha>" and invar +
+    fixes complement :: "'nfa \<Rightarrow> 'nfa"
+    assumes complement_correct:
+      "invar n \<Longrightarrow> invar (complement n)"
+      "invar n \<Longrightarrow> (\<alpha> (complement n) = DFA_complement (\<alpha> n))"
+  begin
+    lemma complement_correct___isomorphic :
+      "invar n \<Longrightarrow> invar (complement n)"
+      "invar n \<Longrightarrow> NFA_isomorphic_wf (\<alpha> n) (\<A> :: ('q2, 'a) NFA_rec) \<Longrightarrow>
+                    NFA_isomorphic_wf (\<alpha> (complement n)) (DFA_complement \<A>)"
+      apply (simp add: complement_correct)
+      apply (insert complement_correct(2)[of n] 
+                  NFA_isomorphic_wf___DFA_complement_cong [of "\<alpha> n" \<A>])
+      apply (simp)
+    done
+end
+
+
+  subsection \<open>  Record Based Interface \<close>
+
+  record ('q,'a, 'b, 'nfa) nfa_ops =
+    nfa_op_\<alpha> :: "('q::{NFA_states},'a,'nfa) nfa_\<alpha>"
+    nfa_op_invar :: "'nfa \<Rightarrow> bool"
+    nfa_op_ba_wf :: "('q list \<times> ('q \<times> 'b \<times> 'q) list 
+      \<times> 'q list \<times> 'q list) \<Rightarrow> bool"
+    nfa_op_bool_comb :: "(bool \<Rightarrow> bool \<Rightarrow> bool) \<Rightarrow> 'nfa \<Rightarrow> 'nfa \<Rightarrow> 'nfa"
+    nfa_op_concate :: "'nfa \<Rightarrow> 'nfa \<Rightarrow> 'nfa"
+ 
+
+  locale StdNFADefs =
+    fixes ops :: "('q::{NFA_states},'a ::linorder, 'b, 'nfa) nfa_ops"
+  begin
+    abbreviation \<alpha> where "\<alpha> \<equiv> nfa_op_\<alpha> ops"
+    abbreviation invar where "invar \<equiv> nfa_op_invar ops"
+    abbreviation nfa_ba_wf where "nfa_ba_wf \<equiv> nfa_op_ba_wf ops"
+(*  abbreviation nfa_from_list where "nfa_from_list \<equiv> nfa_op_nfa_from_list ops" *)
+(*    abbreviation dfa_from_list where "dfa_from_list \<equiv> nfa_op_dfa_from_list ops"
+    abbreviation to_list where "to_list \<equiv> nfa_op_to_list ops"
+    abbreviation accept where "accept \<equiv> nfa_op_accept ops"
+    abbreviation is_deterministic where "is_deterministic \<equiv> nfa_op_is_deterministic ops"
+    abbreviation rename_labels where "rename_labels \<equiv> nfa_op_rename_labels ops"
+    abbreviation normalise where "normalise \<equiv> nfa_op_normalise ops"
+    abbreviation reverse where "reverse \<equiv> nfa_op_reverse ops"
+    abbreviation complement where "complement \<equiv> nfa_op_complement ops"
+    abbreviation bool_comb where "bool_comb \<equiv> nfa_op_bool_comb ops"
+    abbreviation product where "product \<equiv> bool_comb (\<and>)"
+    abbreviation determinise where "determinise \<equiv> nfa_op_determinise ops"
+    abbreviation minimise_Brzozowski where "minimise_Brzozowski \<equiv> nfa_op_minimise_Brzozowski ops"
+    abbreviation minimise_Hopcroft where "minimise_Hopcroft \<equiv> nfa_op_minimise_Hopcroft ops"
+    abbreviation minimise_Hopcroft_NFA where "minimise_Hopcroft_NFA \<equiv> nfa_op_minimise_Hopcroft_NFA ops"
+    abbreviation right_quotient_lists where "right_quotient_lists \<equiv> nfa_op_right_quotient_lists ops"
+    abbreviation states_no where "states_no \<equiv> nfa_op_states_no ops"
+    abbreviation labels_no where "labels_no \<equiv> nfa_op_labels_no ops"
+    abbreviation trans_no where "trans_no \<equiv> nfa_op_trans_no ops"
+    abbreviation initial_no where "initial_no \<equiv> nfa_op_initial_no ops"
+    abbreviation final_no where "final_no \<equiv> nfa_op_final_no ops" *)
+end
+
+
+
+  locale StdNFA = StdNFADefs +
+    nfa \<alpha> invar 
+    (* nfa_from_list \<alpha> invar nfa_from_list + *)
+
+(*
+    nfa_to_list \<alpha> invar to_list +
+    nfa_stats \<alpha> invar states_no trans_no initial_no final_no +
+    nfa_accept \<alpha> invar accept +
+    nfa_rename_labels \<alpha> invar \<alpha> invar rename_labels +
+    nfa_normalise \<alpha> invar normalise +
+    nfa_reverse \<alpha> invar \<alpha> invar reverse +
+    nfa_bool_comb_same \<alpha> invar bool_comb *)
+  begin
+  
+ 
+  end
+end
